examples/tactics/CanonCommMonoid.fst
@@ -1,0 +1,184 @@
+module CanonCommMonoid
+
+open FStar.List
+open FStar.Tactics
+open FStar.Reflection
+
+(* An expression canonizer for commutative monoids
+   Inspired by:
+   - http://adam.chlipala.net/cpdt/html/Cpdt.Reflection.html
+   - http://poleiro.info/posts/2015-04-13-writing-reflective-tactics.html
+*)
+
+(** *** Commutative monoids *)
+
+(* Should eventually go to standard library *)
+
+let right_unitality_lemma (a:Type) (u:a) (mult:a -> a -> a) =
+  x:a -> Lemma (x `mult` u == x)
+
+let left_unitality_lemma (a:Type) (u:a) (mult:a -> a -> a) =
+  x:a -> Lemma (u `mult` x == x)
+
+let associativity_lemma (a:Type) (mult:a -> a -> a) =
+  x:a -> y:a -> z:a -> Lemma (x `mult` y `mult` z == x `mult` (y `mult` z))
+
+let commutativity_lemma (a:Type) (mult:a -> a -> a) =
+  x:a -> y:a -> Lemma (x `mult` y == y `mult` x)
+
+unopteq
+type cm (a:Type) =
+  | CM :
+    unit:a ->
+    mult:(a -> a -> a) ->
+    right_unitality:right_unitality_lemma a unit mult ->
+    left_unitality:left_unitality_lemma a unit mult ->
+    associativity:associativity_lemma a mult ->
+    commutativity:commutativity_lemma a mult ->
+    cm a
+
+let int_plus_cm : cm int =
+  CM 0 (+) (fun x -> ()) (fun x -> ()) (fun x y z -> ()) (fun x y -> ())
+
+(** *** Expression syntax *)
+
+let var = nat
+let vmap (a:Type) = var -> a
+
+type exp : Type =
+  | Unit : exp
+  | Var : var -> exp
+  | Mult : exp -> exp -> exp
+
+let rec exp_to_string (e:exp) =
+  match e with
+  | Unit -> "Unit"
+  | Var x -> "Var " ^ string_of_int x
+  | Mult e1 e2 -> "Mult (" ^ exp_to_string e1
+                   ^ ") (" ^ exp_to_string e2 ^ ")"
+
+let rec mdenote (#a:Type) (m:cm a) (vars:vmap a) (e:exp) : a =
+  match e with
+  | Unit -> CM?.unit m
+  | Var x -> vars x
+  | Mult e1 e2 -> CM?.mult m (mdenote m vars e1) (mdenote m vars e2)
+
+let rec xsdenote (#a:Type) (m:cm a) (vars:vmap a) (xs:list var) : a =
+  match xs with
+  | [] -> CM?.unit m
+  | [x] -> vars x
+  | x::xs' -> CM?.mult m (vars x) (xsdenote m vars xs')
+
+let rec flatten (e:exp) : list var =
+  match e with
+  | Unit -> []
+  | Var x -> [x]
+  | Mult e1 e2 -> flatten e1 @ flatten e2
+
+let rec flatten_correct_aux (#a:Type) (m:cm a) (vars:vmap a) (xs1 xs2:list var) :
+  Lemma (xsdenote m vars (xs1 @ xs2) == CM?.mult m (xsdenote m vars xs1)
+                                                   (xsdenote m vars xs2)) =
+  match xs1 with
+  | [] -> CM?.left_unitality m (xsdenote m vars xs2)
+  | [x] -> if (Nil? xs2) then CM?.right_unitality m (vars x)
+  | x::xs1' -> (CM?.associativity m (vars x) (xsdenote m vars xs1')
+                                             (xsdenote m vars xs2);
+                flatten_correct_aux m vars xs1' xs2)
+
+ let rec flatten_correct (#a:Type) (m:cm a) (vars:vmap a) (e:exp) :
+    Lemma (mdenote m vars e == xsdenote m vars (flatten e)) =
+  match e with
+  | Unit | Var _ -> ()
+  | Mult e1 e2 -> flatten_correct_aux m vars (flatten e1) (flatten e2);
+                  flatten_correct m vars e1; flatten_correct m vars e2
+
+let monoid_reflect (#a:Type) (m:cm a) (vars:vmap a) (e1 e2:exp)
+    (_ : squash (xsdenote m vars (flatten e1) == xsdenote m vars (flatten e2)))
+    : squash (mdenote m vars e1 == mdenote m vars e2) =
+  flatten_correct m vars e1; flatten_correct m vars e2
+
+(* Finds the position of first occurrence of x in xs;
+   this could use eqtype and be completely standard if term provided it *)
+let rec where_aux (n:nat) (x:term) (xs:list term) : Tot (option nat)
+                                                        (decreases xs) =
+  match xs with
+  | [] -> None
+  | x'::xs' -> if term_eq x x' then Some n else where_aux (n+1) x xs'
+let where = where_aux 0
+
+// This expects that mult, unit, and t have already been normalized
+let rec reification_aux (#a:Type) (ts:list term) (vars:vmap a)
+    (mult unit t : term) : Tac (exp * list term * vmap a) =
+  let hd, tl = collect_app_ref t in
+  let tl = list_unref tl in
+  let fvar (t:term) (ts:list term) (vars:vmap a) : Tac (exp * list term * vmap a) =
+    match where t ts with
+    | Some v -> (Var v, ts, vars)
+    | None -> let vfresh = length ts in let z = unquote t in
+              (Var vfresh, ts @ [t],
+                (fun (v:var) -> if v = vfresh then z else vars v))
+  in
+  match inspect hd, tl with
+  | Tv_FVar fv, [(t1, Q_Explicit) ; (t2, Q_Explicit)] ->
+    if term_eq (pack (Tv_FVar fv)) mult
+    then (let (e1,ts,vars) = reification_aux ts vars mult unit t1 in
+          let (e2,ts,vars) = reification_aux ts vars mult unit t2 in
+          (Mult e1 e2, ts, vars))
+    else fvar t ts vars
+  | _, _ ->
+    if term_eq t unit
+    then (Unit, ts, vars)
+    else fvar t ts vars
+
+// TODO: could guarantee same-length lists 
+let reification (#a:Type) (m:cm a) (ts:list term) : Tac (list exp * vmap a) =
+    let mult = norm_term [delta] (quote (CM?.mult m)) in
+    let unit = norm_term [delta] (quote (CM?.unit m)) in
+    let ts   = Tactics.Derived.map (norm_term [delta]) ts in
+    // dump ("mult = " ^ term_to_string mult ^
+    //     "; unit = " ^ term_to_string unit ^
+    //     ";  t   = " ^ term_to_string t);
+    let vars x = CM?.unit m in
+    let (es,_, vars) =
+      Tactics.Derived.fold_left
+        (fun (es,vs,vars) t ->
+          let (e,vs,vars) = reification_aux vs vars mult unit t in (e::es,vs,vars))
+        ([],[],vars) ts
+    in (List.rev es,vars)
+
+let canon_monoid (#a:Type) (m:cm a) : Tac unit =
+  norm [];
+  let g = cur_goal () in
+  match term_as_formula g with
+  | Comp (Eq (Some t)) t1 t2 ->
+      dump ("t1 =" ^ term_to_string t1 ^
+          "; t2 =" ^ term_to_string t2);
+      if term_eq t (quote a) then
+        match reification m [t1;t2] with
+        | [r1;r2], vars ->
+          dump ("r1=" ^ exp_to_string r1 ^
+              "; r2=" ^ exp_to_string r2);
+          dump ("vars =" ^ term_to_string (quote vars));
+          dump ("haha =" ^ term_to_string (norm_term
+               [delta;primops]
+            (quote (mdenote m vars r1 == mdenote m vars r2))));
+          change_sq (quote (mdenote m vars r1 == mdenote m vars r2));
+          apply (`monoid_reflect);
+          norm [delta_only ["CanonCommMonoid.xsdenote";
+                            "CanonCommMonoid.flatten";
+                            "FStar.List.Tot.Base.op_At";
+                            "FStar.List.Tot.Base.append"]]; dump "done"
+        | _ -> fail "Unexpected"
+      else fail "Goal should be an equality at the right monoid type"
+  | _ -> fail "Goal should be an equality"
+
+let lem0 (a b c d : int) =
+  assert_by_tactic (0 + a + b + c + d == (0 + a) + (b + c + 0) + (d + 0))
+  (fun _ -> canon_monoid int_plus_cm; trefl())
+
+
+(* TODO: would be nice to just find all terms of monoid type in the
+         goal and replace them with their canonicalization;
+         basically use flatten_correct instead of monoid_reflect
+         - even better, the user would have control over the place(s)
+           where the canonicalization is done *)
